theories/Eq/SBisim_draft.v
@@ -1,0 +1,1433 @@
+(*| HS
+Strong bisimilarity
+===================
+
+Companion to [Eq.SSim] / [Eq.CSSim]. [sb L] is the symmetric variant of
+strong simulation:
+
+    sb L R t u  ≜  ss L R t u  ∧  ss (flipL L) (flip R) u t
+
+Its greatest fixed point is [sbisim L], notated [t (σ L) u] (or [t ~ u]
+with the default [eq] relation on labels).
+
+File organisation mirrors [Eq.SSim]:
+- definition of [sb]/[sbisim], notations, folding/step/coinduction/play
+  tactics;
+- homogeneous theory (Reflexive / Symmetric / Transitive / PreOrder /
+  Equivalence, both on [sb L R] and on chain elements);
+- heterogeneous theory: [sbisim_mono], [equ_clos]/[sbisim_clos] up-to
+  principles, [Proper] instances for rewriting [Seq] and [equ eq] on
+  either side, subrelations to [ssim] and [cssim];
+- up-to bind;
+- structural proof rules and inversion principles, using the same
+  [sb_*_gen] / [`R] / [sbisim_*] naming convention as [SSim.v];
+- sanity checks ([spinS], [br2], [brS2] laws) and incompatibility
+  lemmas;
+- interaction with [ss]/[ssim] and [css]/[cssim].
+
+All proofs are [Admitted.] in this draft.
+|*)
+
+From Stdlib Require Import
+     Lia
+     Basics
+     Fin
+     RelationClasses
+     Program.Equality
+     Logic.Eqdep.
+
+From Coinduction Require Import all.
+
+From ITree Require Import Core.Subevent.
+
+From CTree Require Import
+     CTree
+     Utils
+     Eq.Equ
+     Eq.Shallow
+     Eq.Trans
+     Eq.SSim
+     Eq.CSSim.
+
+From RelationAlgebra Require Export
+     rel srel.
+
+Import CoindNotations.
+Import CTree.
+Set Implicit Arguments.
+
+(*|
+Definition
+----------
+|*)
+Section StrongBisim.
+  Context {E F C D : Type -> Type} {X Y : Type}.
+
+  Program Definition sb (L : lrel E F X Y) :
+    mon (@S E C X -> @S F D Y -> Prop) :=
+    {| body R t u := ss L R t u /\ ss (flipL L) (flip R) u t |}.
+  Next Obligation.
+    split; intros; [edestruct H0 as (? & ? & ?) | edestruct H1 as (? & ? & ?)]; eauto; eexists; eexists; intuition; eauto.
+  Qed.
+
+  #[global] Instance lequiv_sb : Proper (lequiv ==> weq) sb.
+  Proof.
+    cbn -[sb]. intros * EQ *; split.
+    - intros [For Bac]; split.
+      eapply lequiv_ss in EQ.
+      now apply EQ in For.
+      eapply lequiv_ss; [| eauto].
+      now apply lequiv_flipL.
+    - intros [For Bac]; split.
+      eapply lequiv_ss; eauto.
+      eapply lequiv_ss; [| eauto].
+      now apply lequiv_flipL.
+  Qed.
+
+End StrongBisim.
+
+Definition sbisim {E F C D X Y} L :=
+  (gfp (@sb E F C D X Y L) : hrel _ _).
+
+Module SBisimNotations.
+
+  Notation sbisimeq := (sbisim Leq).
+  Infix "≃" := (sbisim Leq) (at level 70).
+  Notation "t (≃ [ Q ] ) u" := (sbisim (Lvrel Q) t u) (at level 79).
+  Notation "t (≃ L ) u" := (sbisim L t u) (at level 79).
+
+  Notation "t '[≃]' u" := (sb Leq (` _) t u) (at level 90, only printing).
+  Notation "t '[≃' [ R ] ']' u" := (sb (Lvrel R) (` _) t u) (at level 90, only printing).
+  Notation "t '[≃' R ']' u" := (sb R (` _) t u) (at level 90, only printing).
+
+End SBisimNotations.
+
+Import SBisimNotations.
+Import CTreeNotations.
+Import EquNotations.
+
+(*|
+Hook letting [coq-coinduction]'s symmetric tactic fire on homogeneous
+bisimulations.
+|*)
+#[global] Instance sbisim_sym {E C X L} :
+  Symmetric L ->
+  Symmetrical converse (@sb E E C C X X (Lvrel L)) (@ss E E C C X X (Lvrel L)).
+Proof.
+  intros SYM. intros RR u v. split; intros HSIM.
+  - destruct HSIM as [F B]. split.
+    + apply F.
+    + cbn. intros l v' TR.
+      apply B in TR as (l' & u' & TR & HR & HR').
+      ex2; split3; eauto.
+      symmetry.
+      pose proof flipL_flip (Lvrel L) l l' as G.
+      now apply G.
+  - destruct HSIM as [F B]. split.
+    + apply F.
+    + intros l v' TR.
+      apply B in TR as (l' & u' & TR & HR & HR').
+      ex2; split3; eauto.
+      pose proof flipL_flip (Lvrel L) l l' as G.
+      apply G.
+      now symmetry.
+Qed.
+
+(*|
+Tactics
+-------
+|*)
+Ltac fold_sbisim :=
+  repeat
+    match goal with
+    | h: context[gfp (@sb ?E ?F ?C ?D ?X ?Y ?L)] |- _ => fold (@sbisim E F C D X Y L) in h
+    | |- context[gfp (@sb ?E ?F ?C ?D ?X ?Y ?L)]      => fold (@sbisim E F C D X Y L)
+    end.
+
+Tactic Notation "__step_sbisim" :=
+  match goal with
+  | |- context[@sbisim ?E ?F ?C ?D ?X ?Y ?LR] =>
+      unfold sbisim;
+      step;
+      fold (@sbisim E F C D X Y L)
+  end.
+#[local] Tactic Notation "step" := __step_sbisim || __step_cssim || __step_ssim || step.
+
+Ltac __step_in_sbisim H :=
+  match type of H with
+  | context[@sbisim ?E ?F ?C ?D ?X ?Y ?LR] =>
+      unfold sbisim in H;
+      step in H;
+      fold (@sbisim E F C D X Y L) in H
+  end.
+#[local] Tactic Notation "step" "in" ident(H) := __step_in_sbisim H || step in H.
+
+Tactic Notation "__coinduction_sbisim" simple_intropattern(r) simple_intropattern(cih) :=
+  first [unfold sbisim at 4 | unfold sbisim at 3 | unfold sbisim at 2 | unfold sbisim at 1]; coinduction r cih.
+#[local] Tactic Notation "coinduction" simple_intropattern(r) simple_intropattern(cih) :=
+  __coinduction_sbisim r cih || __coinduction_cssim r cih || __coinduction_ssim r cih || coinduction r cih.
+
+Ltac __play_sbisim := (try step); split; cbn; intros ? ? ?TR.
+
+Ltac __playL_sbisim H :=
+  (try step in H);
+  let Hf := fresh "Hf" in
+  destruct H as [Hf _];
+  cbn in Hf; edestruct Hf as (? & ? & ?TR & ?EQ & ?);
+  clear Hf; [etrans |].
+
+Ltac __playR_sbisim H :=
+  (try step in H);
+  let Hb := fresh "Hb" in
+  destruct H as [_ Hb];
+  cbn in Hb; edestruct Hb as (? & ? & ?TR & ?EQ & ?);
+  clear Hb; [etrans |].
+
+Ltac __eplayL_sbisim :=
+  match goal with
+  | h : @sbisim ?E _ ?C _ ?X _ ?RR _ _ |- _ => __playL_sbisim h
+  | h : body (sb ?L) ?R _ _ |- _ => __playL_sbisim h
+  end.
+
+Ltac __eplayR_sbisim :=
+  match goal with
+  | h : @sbisim ?E _ ?C _ ?X _ ?RR _ _ |- _ => __playR_sbisim h
+  | h : body (sb ?L) ?R _ _ |- _ => __playR_sbisim h
+  end.
+
+Ltac __answer_sbisim := ex2; split3; etrans.
+
+#[local] Tactic Notation "play"                 := __play_sbisim.
+#[local] Tactic Notation "playL" "in" ident(H)  := __playL_sbisim H.
+#[local] Tactic Notation "playR" "in" ident(H)  := __playR_sbisim H.
+#[local] Tactic Notation "play"  "in" ident(H)  := first [playL in H; [] | playR in H; []].
+#[local] Tactic Notation "eplayL"               := __eplayL_sbisim.
+#[local] Tactic Notation "eplayR"               := __eplayR_sbisim.
+#[local] Tactic Notation "eplay"                := first [eplayL; [] | eplayR; []].
+#[local] Tactic Notation "answer"               := __answer_sbisim.
+
+(*|
+Homogeneous theory
+------------------
+|*)
+Section sbisim_homogenous_theory.
+  Context {E B : Type -> Type} {X : Type}
+          {L : lrel E E X X}.
+
+  Notation sb    := (@sb    E E B B X X).
+  Notation sbisim := (@sbisim E E B B X X).
+
+  #[global] Instance reflexive_sb {R}
+    (LR : Reflexive L) (RR : Reflexive R) : Reflexive (sb L R).
+  Proof.
+    split. reflexivity.
+    cbn; eauto 10.
+  Qed.
+
+  #[global] Instance reflexive_chain {LR : Reflexive L} {C : Chain (sb L)} : Reflexive `C.
+  Proof.
+    apply Reflexive_chain; typeclasses eauto.
+  Qed.
+
+  #[global] Instance symmetric_sb {R}
+    (LS : Symmetric L) (RS : Symmetric R) : Symmetric (sb L R).
+  Proof.
+    intros u v SB.
+    play; eplay.
+    answer; now apply flipL_flip.
+    answer; now apply flipL_flip.
+  Qed.
+
+  #[global] Instance symmetric_chain {LS : Symmetric L} {C : Chain (sb L)} : Symmetric `C.
+  Proof.
+    apply Symmetric_chain; typeclasses eauto.
+  Qed.
+
+  #[global] Instance transitive_sb {R}
+    (LT : Transitive L) (RT : Transitive R) : Transitive (sb L R).
+  Proof.
+    intros x y z SS1 SS2.
+    play.
+    - play in SS1; play in SS2; answer.
+    - play in SS2; play in SS1; answer.
+      apply (flipL_flip L) in H,H0; apply flipL_flip; cbn in *; eauto.
+  Qed.
+
+  #[global] Instance transitive_chain {LT : Transitive L} {C : Chain (sb L)} : Transitive `C.
+  Proof.
+    apply Transitive_chain; typeclasses eauto.
+  Qed.
+
+  #[global] Instance preOrder_sb {R}
+    (LE : PreOrder L) (RE : PreOrder R) : PreOrder (sb L R).
+  Proof. split; typeclasses eauto. Qed.
+
+  #[global] Instance PreOrder_chain {LPO : PreOrder L} {C : Chain (sb L)} : PreOrder `C.
+  Proof. split; typeclasses eauto. Qed.
+
+  #[global] Instance equivalence_sb {R}
+    (LE : Equivalence L) (RE : Equivalence R) : Equivalence (sb L R).
+  Proof. split; typeclasses eauto. Qed.
+
+  #[global] Instance equivalence_chain {LE : Equivalence L} {C : Chain (sb L)} : Equivalence `C.
+  Proof. split; typeclasses eauto. Qed.
+
+End sbisim_homogenous_theory.
+
+Lemma Leq_eq {E X}: build_rel (@Leq E X) == eq.
+Proof.
+  split; [| intros <-; reflexivity].
+  intros []; auto.
+  dependent induction HR; auto.
+  dependent induction HR; auto.
+  cbn in H; subst; auto.
+Qed.
+
+Lemma flipL_Leq {E X}: lequiv (flipL (@Leq E X)) Leq.
+Proof.
+  cbv; intuition.
+  all: dependent induction H; constructor.
+Qed.
+
+(*|
+Heterogeneous theory
+--------------------
+|*)
+Section sbisim_heterogenous_theory.
+  Arguments label : clear implicits.
+  Context {E F C D : Type -> Type} {X Y : Type}.
+
+  Notation sb     := (@sb     E F C D X Y).
+  Notation sbisim := (@sbisim E F C D X Y).
+
+  Lemma sbisim_mono : Proper (sub_lrel ==> leq) sbisim.
+  Proof. 
+    cbn; intros RR SS SUB.
+    coinduction R cih.
+    intros u v HSB; split.
+    - intros ? ? TR; eplay; answer.
+      eapply sub_lrel_subrel; eauto.
+    - intros ? ? TR; cbn.
+      eplay. answer.
+      apply lequiv_sub_lrel in SUB.
+      eapply sub_lrel_subrel; eauto.
+  Qed.
+
+  Context {L : lrel E F X Y}.
+
+  (*| Up-to [equ_clos]. |*)
+  (* Lemma equ_clos_chain {c : Chain (sb L)} : *)
+  (*   forall x y, equ_clos `c x y -> `c x y. *)
+  (* Proof. *)
+  (*   apply tower. *)
+  (*   - intros ? INC x y [x' y' x'' y'' EQ' EQ''] ??. red. *)
+  (*     apply INC; auto. *)
+  (*     econstructor; eauto. *)
+  (*     apply leq_infx in H. *)
+  (*     now apply H. *)
+  (*   - clear. *)
+  (*     intros c IH x y []; split. *)
+  (*     + intros l z x'z. *)
+  (*       rewrite Equt in x'z. *)
+  (*       apply HR in x'z as (? & ? & ? & ? & ?). *)
+  (*       do 2 eexists; intuition; eauto. *)
+  (*       rewrite <- Equu; eauto. *)
+  (*     + intros l z x'z. *)
+  (*       rewrite <- Equu in x'z. *)
+  (*       apply HR in x'z as (? & ? & ? & ? & ?). *)
+  (*       do 2 eexists; intuition; eauto. *)
+  (*       rewrite Equt; eauto. *)
+  (* Qed. *)
+
+  #[global] Instance seq_chain_goal {c : Chain (sb L)} :
+    Proper (Seq ==> Seq ==> flip impl) `c.
+  Proof.
+    apply tower.
+    - intros ? INC t t' HP' ? ? HP'' ?? HP'''. 
+      red.
+      eapply INC; eauto.
+      apply leq_infx in HP'''.
+      now apply HP'''.
+    - intros ? INC  t t' EQt u u' EQu HBS; split; intros l v TR.
+      + rewrite EQt in TR.
+        eplay.
+        answer.
+        now rewrite EQu.
+      + rewrite EQu in TR.
+        eplay.
+        answer.
+        now rewrite EQt.
+  Qed.
+
+  #[global] Instance equ_chain_goal {c : Chain (sb L)} :
+    Proper (equ eq ==> equ eq ==> flip impl) `c.
+  Proof.
+    repeat intro; eapply seq_chain_goal; [| |eauto]; eauto.
+  Qed.
+
+  #[global] Instance seq_sb_goal {r} :
+    Proper (Seq ==> Seq ==> flip impl) (sb L r).
+  Proof.  
+    intros t t' tt' u u' uu' HBS; split; intros ?? TR.
+    - rewrite tt' in TR.
+      eplay; answer.
+      now rewrite uu'.
+    - rewrite uu' in TR.
+      eplay; answer.
+      now rewrite tt'.
+  Qed.  
+  
+  #[global] Instance equ_sb_goal {r} :
+    Proper (equ eq ==> equ eq ==> flip impl) (sb L r).
+  Proof.
+    repeat intro; eapply seq_sb_goal; [| | eauto]; eauto.
+  Qed.
+  
+  #[global] Instance sbisim_chain_goal {c : Chain (sb L)} :
+    Proper (sbisimeq ==> sbisimeq ==> flip impl) `c.
+  Proof.
+    apply tower.
+    - intros ? INC t t' HP' ? ? HP'' ?? HP'''. 
+      red.
+      eapply INC; eauto.
+      apply leq_infx in HP'''.
+      now apply HP'''.
+    - intros ? INC  t t' Sbisimt u u' Sbisimu [fwd bwd]; split; intros l v TR.
+      + step in Sbisimt; apply Sbisimt in TR; destruct TR as (? & ? & TR & Sbis & EQl).
+        apply fwd in TR; destruct TR as (? & ? & TR & Sbis' & HL).
+        step in Sbisimu; apply Sbisimu in TR; destruct TR as (? & ? & TR & Sbis'' & EQl').
+        do 2 eexists; repeat split; eauto.
+        eapply INC; eauto.
+        (* todo ltac *)
+        apply Leq_eq in EQl.
+        rewrite flipL_Leq in EQl'.
+        apply Leq_eq in EQl'.
+        subst; auto.
+      + step in Sbisimu; apply Sbisimu in TR; destruct TR as (? & ? & TR & Sbis & EQl).
+        apply bwd in TR; destruct TR as (? & ? & TR & Sbis' & HL).
+        step in Sbisimt; apply Sbisimt in TR; destruct TR as (? & ? & TR & Sbis'' & EQl').
+        do 2 eexists; repeat split; eauto.
+        eapply INC; eauto.
+        apply Leq_eq in EQl.
+        rewrite flipL_Leq in EQl'.
+        apply Leq_eq in EQl'.
+        subst; auto.
+  Qed.
+   
+  #[global] Instance seq_chain_ctx {c : Chain (sb L)} :
+    Proper (Seq ==> Seq ==> impl) `c.
+  Proof.
+    apply tower.
+    - intros ? INC t t' HP' ? ? HP'' ?? HP'''. 
+      red.
+      eapply INC; eauto.
+      apply leq_infx in HP'''.
+      now apply HP'''.
+    - intros ? INC  t t' EQt u u' EQu HBS; split; intros l v TR.
+      + rewrite <- EQt in TR.
+        eplay.
+        answer.
+        now rewrite <- EQu.
+      + rewrite <- EQu in TR.
+        eplay.
+        answer.
+        now rewrite <- EQt.
+  Qed.
+
+  #[global] Instance equ_chain_ctx {c : Chain (sb L)} :
+    Proper (equ eq ==> equ eq ==> impl) `c.
+  Proof.
+    repeat intro; eapply seq_chain_ctx; [| | eauto]; eauto.
+  Qed.
+
+  #[global] Instance seq_sb_ctx {r} :
+    Proper (Seq ==> Seq ==> impl) (sb L r).
+  Proof.
+    intros t t' tt' u u' uu' HBS; split; intros ?? TR.
+    - rewrite <- tt' in TR.
+      eplay; answer.
+      now rewrite <- uu'.
+    - rewrite <- uu' in TR.
+      eplay; answer.
+      now rewrite <- tt'.
+  Qed.  
+
+  #[global] Instance equ_sb_ctx {r} :
+    Proper (equ eq ==> equ eq ==> impl) (sb L r).
+  Proof.
+    repeat intro; eapply seq_sb_ctx; [| | eauto]; eauto.
+  Qed.
+  
+  #[global] Instance sbisim_chain_ctx {c : Chain (sb L)} :
+    Proper (sbisimeq ==> sbisimeq ==> impl) `c.
+  Proof.
+    apply tower.
+    - intros ? INC t t' HP' ? ? HP'' ?? HP'''. 
+      red.
+      eapply INC; eauto.
+      apply leq_infx in HP'''.
+      now apply HP'''.
+    - intros ? INC  t t' Sbisimt u u' Sbisimu [fwd bwd]; split; intros l v TR.
+      + step in Sbisimt; apply Sbisimt in TR; destruct TR as (? & ? & TR & Sbis & EQl).
+        apply fwd in TR; destruct TR as (? & ? & TR & Sbis' & HL).
+        step in Sbisimu; apply Sbisimu in TR; destruct TR as (? & ? & TR & Sbis'' & EQl').
+        do 2 eexists; repeat split; eauto.
+        eapply INC; eauto.
+        (* todo ltac *)
+        apply Leq_eq in EQl'.
+        rewrite flipL_Leq in EQl.
+        apply Leq_eq in EQl.
+        subst; auto.
+      + step in Sbisimu; apply Sbisimu in TR; destruct TR as (? & ? & TR & Sbis & EQl).
+        apply bwd in TR; destruct TR as (? & ? & TR & Sbis' & HL).
+        step in Sbisimt; apply Sbisimt in TR; destruct TR as (? & ? & TR & Sbis'' & EQl').
+        do 2 eexists; repeat split; eauto.
+        eapply INC; eauto.
+        apply Leq_eq in EQl'.
+        rewrite flipL_Leq in EQl.
+        apply Leq_eq in EQl.
+        subst; auto.
+  Qed.
+  
+  (*| Subrelations. |*)
+
+  Lemma sbisim_cssim_subrelation_gen :
+    forall x y, sbisim L x y -> cssim L x y.
+  Proof.
+    red.
+    coinduction r cih; intros * SB.
+    step in SB; destruct SB as [fwd bwd].
+    split.
+    - intros ?? TR; apply fwd in TR as (? & ? & ? & ? & ?); eauto 10.
+    - intros (? & ? & TR). apply bwd in TR as (? & ? & ? & ? & ?); eauto 10.
+  Qed.
+
+  Lemma sbisim_ssim_subrelation_gen :
+    forall x y, sbisim L x y -> ssim L x y.
+  Proof. 
+    intros. now apply cssim_ssim_subrelation_gen, sbisim_cssim_subrelation_gen.
+  Qed.
+  
+End sbisim_heterogenous_theory.
+
+(* TODO (?) : generalize
+Lemma equ_sbisim_subrelation_gen {E B X Y} (RR : rel X Y) :
+  forall x y, SeqR RR x y -> @sbisim E E B B X Y (Lvrel RR) x y.
+ *)
+
+#[global] Instance equ_sbisim_subrelation {E B X} :
+  subrelation (@Seq E B X) sbisimeq.
+Proof.
+  red; intros * EQ; now rewrite EQ.
+Qed.
+
+#[global] Instance sbisim_cssim_subrelation {E C X L} :
+  subrelation (@sbisim E E C C X X L) (cssim L).
+Proof.
+  red; apply sbisim_cssim_subrelation_gen. 
+Qed.
+
+#[global] Instance sbisim_ssim_subrelation {E C X L} :
+  subrelation (@sbisim E E C C X X L) (ssim L).
+Proof.
+  red; apply sbisim_ssim_subrelation_gen. 
+Qed.
+
+#[global] Instance weq_sbisim : forall {E F C D X Y},
+    Proper (lequiv ==> weq) (@sbisim E F C D X Y).
+Proof.
+    cbn -[weq]. intros. apply gfp_weq. now apply lequiv_sb.
+Qed.
+
+#[global] Instance is_stuck_sbisim_iff {E C X L} :
+  Proper (@sbisim E E C C X X L ==> iff) is_stuck.
+Proof.
+  cbn; split; intros IS ?? TR.
+  all:step in H; destruct H as [fwd bwd].
+  apply bwd in TR as (? & ? & ? & ? & ?); eapply IS; eauto.
+  apply fwd in TR as (? & ? & ? & ? & ?); eapply IS; eauto.
+Qed.
+
+(*|
+Up-to bind
+----------
+|*)
+Section bind.
+  Arguments label : clear implicits.
+  Obligation Tactic := idtac.
+
+  Lemma bind_chain_gen
+    {E F C D : Type -> Type} {X X' Y Y' : Type}
+    (L  : lrel E F X' Y')
+    (SS : rel X Y)
+    {R : Chain (@sb E F C D X' Y' L)} :
+    forall (t : ctree E C X) (t' : ctree F D Y)
+      (k : X -> ctree E C X') (k' : Y -> ctree F D Y'),
+      sbisim (upd_rel L SS) t t' ->
+      (forall x y, SS x y -> `R (k x) (k' y)) ->
+      `R (bind t k) (bind t' k').
+  Proof.
+    apply tower.
+    - intros ? INC ? ? ? ? tt' kk' ? ?.
+      apply INC. apply H. apply tt'.
+      intros x x' xx'. apply leq_infx in H. apply H. now apply kk'.
+    - intros ? ? ? ? ? ? tt' kk'.
+      step in tt'; destruct tt' as [fwd bwd].
+      split; cbn; intros * STEP.
+      + apply trans_bind_inv in STEP as [(?H & ?t' & STEP & EQ) | [(Z & e & EQl & g & STEP & SEQ) | (v & STEPres & STEP)]].
+        * subst l.
+          apply fwd in STEP as (? & ? & STEP' & HSIM & HRL).
+          inv HRL.
+          refine_trans.
+          ex2; split3.
+          apply trans_bind_l_τ; eauto.
+          2: etrans.
+          rewrite EQ.
+          apply H; auto.
+          intros.
+          now step; apply kk'.
+        * subst l.
+          apply fwd in STEP as (? & ? & STEP' & HSIM & HRL).
+          invL.
+          refine_trans.
+          exists (ask f); ex; split3.
+          eapply trans_bind_l_ask; eauto.
+          2:etrans.
+          rewrite SEQ.
+          step; split.
+          all: intros ? ? STEP''.
+          all: pose proof trans_passive_inv' STEP'' as (a & EQ & ->).
+          all: rewrite EQ in STEP''.
+          assert (TR: trans (rcv e a) (β e g) (g a)) by etrans.
+          2:assert (TR: trans (rcv f a) (β f u) (u a)) by etrans.
+          all:step in HSIM; apply HSIM in TR as (l' & u' & TR' & HSIM' & HRL').
+          all:pose proof trans_passive_inv' TR' as (b & EQ' & ->).
+          exists (rcv f b); ex; split; eauto; split; cycle 1; [invL; etrans |].
+          2:exists (rcv e b); ex; split; eauto; split; cycle 1; [invL; etrans |].
+          all:rewrite EQ.
+          all:apply H.
+          1,3:rewrite EQ' in HSIM'; auto.
+          all:intros; now step; apply kk'.
+        * apply fwd in STEPres as (? & ? & STEP' & HSIM & HRL).
+          invL.
+          apply (kk' v y) in STEP as (l' & u' & STEP'' & HSIM'' & HRL'); etrans.
+          exists l'; eexists; split; eauto.
+          eapply trans_bind_r; eauto.
+          erewrite <- trans_val_inv'; eauto.
+       + apply trans_bind_inv in STEP as [(?H & ?t' & STEP & EQ) | [(Z & e & EQl & g & STEP & SEQ) | (v & STEPres & STEP)]].
+        * subst l.
+          apply bwd in STEP as (? & ? & STEP' & HSIM & HRL).
+          inv HRL.
+          refine_trans.
+          ex2; split3.
+          apply trans_bind_l_τ; eauto.
+          2: etrans.
+          rewrite EQ.
+          apply H; auto.
+          intros.
+          now step; apply kk'.
+        * subst l.
+          apply bwd in STEP as (? & ? & STEP' & HSIM & HRL).
+          invL.
+          refine_trans.
+          exists (ask f); ex; split3.
+          eapply trans_bind_l_ask; eauto.
+          2:etrans.
+          rewrite SEQ.
+          step; split.
+          all: intros ? ? STEP''.
+          all: pose proof trans_passive_inv' STEP'' as (a & EQ & ->).
+          all: rewrite EQ in STEP''.
+          assert (TR: trans (rcv f a) (β f u) (u a)) by etrans.
+          2:assert (TR: trans (rcv e a) (β e g) (g a)) by etrans.
+          all:step in HSIM; apply HSIM in TR as (l' & u' & TR' & HSIM' & HRL').
+          all:pose proof trans_passive_inv' TR' as (b & EQ' & ->).
+          exists (rcv e b); ex; split; eauto; split; cycle 1; [invL; etrans |].
+          2:exists (rcv f b); ex; split; eauto; split; cycle 1; [invL; etrans |].
+          all:rewrite EQ.
+          all:apply H.
+          1,3:rewrite EQ' in HSIM'; auto.
+          all:intros; now step; apply kk'.
+        * apply bwd in STEPres as (? & ? & STEP' & HSIM & HRL).
+          invL.
+          eapply (kk' _ _) in STEP as (l' & u' & STEP'' & HSIM'' & HRL'); etrans.
+          exists l'; eexists; split; eauto.
+          eapply trans_bind_r; eauto.
+          erewrite <- trans_val_inv'; eauto.
+  Qed.
+
+  Lemma bind_chain {E C D X Y X' Y'}
+    (RR : rel X' Y') (SS : rel X Y)
+    {R : Chain (@sb E E C D X' Y' (Lvrel RR))} :
+    forall (t1 : ctree E C X) (t2 : ctree E D Y) (k1 : X -> ctree E C X') (k2 : Y -> ctree E D Y'),
+      t1 (≃[SS]) t2 ->
+      (forall x y, SS x y -> `R (k1 x) (k2 y)) ->
+      `R (t1 >>= k1) (t2 >>= k2).
+  Proof.
+    intros.
+    eapply bind_chain_gen; eauto.
+  Qed.
+
+  Lemma bind_chain_eq {E C X X'}
+    {R : Chain (@sb E E C C X' X' Leq)} :
+    forall (t1 t2 : ctree E C X)
+           (k1 k2 : X -> ctree E C X'),
+      t1 ≃ t2 ->
+      (forall x, `R (k1 x) (k2 x)) ->
+      `R (t1 >>= k1) (t2 >>= k2).
+  Proof.
+    intros.
+    eapply bind_chain_gen; eauto.
+    intros ??<-; auto.
+  Qed.
+
+  Lemma sbisim_bind_gen {E F C D X Y X' Y'}
+    L (SS : rel X Y)
+    (t1 : ctree E C X) (t2 : ctree F D Y)
+    (k1 : X -> ctree E C X') (k2 : Y -> ctree F D Y') :
+    t1 (≃ upd_rel L SS) t2 ->
+    (forall x y, SS x y -> k1 x (≃ L) k2 y) ->
+    t1 >>= k1 (≃ L) t2 >>= k2.
+  Proof.
+    intros.
+    eapply bind_chain_gen; eauto.
+  Qed.
+
+  Lemma sbisim_bind {E C D X Y X' Y'}
+    (RR : rel X' Y') (SS : rel X Y)
+    (t1 : ctree E C X) (t2 : ctree E D Y)
+    (k1 : X -> ctree E C X') (k2 : Y -> ctree E D Y') :
+    t1 (≃[SS]) t2 ->
+    (forall x y, SS x y -> k1 x (≃[RR]) k2 y) ->
+    t1 >>= k1 (≃[RR]) t2 >>= k2.
+  Proof.
+    intros.
+    eapply bind_chain_gen; eauto.
+  Qed.
+
+  Lemma sbisim_bind_eq {E C D X X'}
+    (t1 : ctree E C X) (t2 : ctree E D X)
+    (k1 : X -> ctree E C X') (k2 : X -> ctree E D X') :
+    t1 ≃ t2 ->
+    (forall x, k1 x ≃ k2 x) ->
+    t1 >>= k1 ≃ t2 >>= k2.
+  Proof.
+    intros.
+    eapply sbisim_bind; eauto.
+    intros ?? ->; auto.
+  Qed.
+
+End bind.
+
+#[global] Instance sbisim_bind_chain {E C X Y}
+  {R : Chain (@sb E E C C Y Y Leq)} :
+  Proper ((fun t u => sbisim Leq (α t) (α u)) ==>
+          (pointwise_relation _ (fun t u => `R (α t) (α u))) ==> `R) (@bind E C X Y).
+Proof.
+  repeat intro; eapply bind_chain_gen; eauto.
+  intros ?? <-; auto.
+Qed.
+
+(*|
+Structural proof rules
+======================
+Same three-layer shape as in [SSim.v] / [CSSim.v]:
+- [sb_*_gen]: body-level, arbitrary [R], side-conditions explicit;
+- [sb_*]: body-level, on a chain element [`R];
+- [sbisim_*]: gfp-level.
+|*)
+Section Proof_Rules.
+
+  Context {E F C D : Type -> Type} {X Y : Type}.
+
+  (*|
+  Stuck ctrees: under bisimilarity the meaningful statement is biconditional.
+  |*)
+  Lemma sb_is_stuck L R :
+    forall (t : ctree E C X) (u : ctree F D Y),
+      sb L R t u -> is_stuck t <-> is_stuck u.
+  Proof.
+    intros * SB; split; intros IS ?? TR; eplay; eapply IS; eauto.
+  Qed.
+  
+  Lemma sbisim_is_stuck L :
+    forall (t : ctree E C X) (u : ctree F D Y),
+      sbisim L t u -> is_stuck t <-> is_stuck u.
+  Proof.
+    intros * SB; step in SB; eauto using sb_is_stuck.
+  Qed.
+  
+  Lemma is_stuck_sb L R :
+    forall (t : ctree E C X) (u : ctree F D Y),
+      is_stuck t -> is_stuck u -> sb L R t u.
+  Proof.  
+    split; repeat intro.
+    - now apply H in H1.
+    - now apply H0 in H1.
+  Qed.
+    
+  Lemma is_stuck_sbisim L :
+    forall (t : ctree E C X) (u : ctree F D Y),
+      is_stuck t -> is_stuck u -> sbisim L t u.
+  Proof.
+    intros; step; auto using is_stuck_sb.
+  Qed.
+
+  Lemma Chain_Stuck L {R : Chain (@sb E F C D X Y L)} :
+    ` R Stuck Stuck.
+  Proof.
+    step. apply is_stuck_sb; auto using stuck_is_stuck.
+  Qed.
+  
+  (*|
+  Ret nodes
+  |*)
+  Lemma sb_ret_gen (x : X) (y : Y) L R :
+    R (α Stuck) (α Stuck) ->
+    (Proper (Seq ==> Seq ==> impl) R) ->
+    RR L x y ->
+    sb L R (Ret x : ctree E C X) (Ret y : ctree F D Y).
+   Proof.
+    intros Rstuck ValRefl PROP.
+    split; apply ss_ret_gen; eauto.
+    typeclasses eauto.
+  Qed.
+
+  Lemma sb_ret (x : X) (y : Y) L
+    {R : Chain (@sb E F C D X Y L)} :
+    RR L x y ->
+    sb L `R (Ret x : ctree E C X) (Ret y : ctree F D Y).
+  Proof.
+    intros; apply sb_ret_gen; auto.
+    apply Chain_Stuck.
+    typeclasses eauto.
+  Qed. 
+
+  Lemma sbisim_ret (x : X) (y : Y) L :
+    RR L x y ->
+    sbisim L (Ret x : ctree E C X) (Ret y : ctree F D Y).
+  Proof.
+    intros; step; now apply sb_ret.
+  Qed.
+
+  (*|
+  Vis nodes
+  |*)
+
+  Lemma sb_vis_gen {Z Z'} (e : E Z) (f: F Z')
+    (k : Z -> ctree E C X) (k' : Z' -> ctree F D Y) (R: rel _ _) (L : lrel E F X Y) :
+    R (β (e) k) (β (f) k') ->
+    (Proper (Seq ==> Seq ==> impl) R) ->
+    L (ask e) (ask f) ->
+    sb L R (Vis e k) (Vis f k').
+  Proof.
+    intros; split; apply ss_vis_gen; try typeclasses eauto; auto.
+    now apply flipL_flip.
+  Qed.
+ 
+  Lemma sb_vis {Z Z'} (e : E Z) (f : F Z')
+    (k : Z -> ctree E C X) (k' : Z' -> ctree F D Y) L
+    {R : Chain (@sb E F C D X Y L)}
+    (HRask : Rask L e f)
+    (HRfwd : forall x, exists y, `R (k x) (k' y) /\ Rrcv L e f x y)
+    (HRbwd : forall y, exists x, `R (k x) (k' y) /\ Rrcv L e f x y) :
+    sb L `R (Vis e k) (Vis f k').
+  Proof.
+    apply sb_vis_gen; try typeclasses eauto.
+    2: now constructor.
+    step; split.
+    all: intros l u TR; inv_trans; subst.
+    destruct (HRfwd x) as (y & ? & ?).
+    2:destruct (HRbwd x) as (y & ? & ?).
+    all:ex2; intuition.
+    rewrite EQ; eauto.
+    etrans.
+    rewrite EQ; eauto.
+    apply flipL_flip; cbn; etrans.
+  Qed.
+
+  Lemma sbisim_vis {Z Z'} (e : E Z) (f : F Z')
+    (k : Z -> ctree E C X) (k' : Z' -> ctree F D Y) L
+    (HRask : Rask L e f)
+    (HRfwd : forall x, exists y, sbisim L (k x) (k' y) /\ Rrcv L e f x y)
+    (HRbwd : forall y, exists x, sbisim L (k x) (k' y) /\ Rrcv L e f x y) :
+    sbisim L (Vis e k) (Vis f k').
+  Proof.
+    now step; apply sb_vis.
+  Qed.
+  
+  Lemma sb_vis_id {Z} (e : E Z) (f : F Z)
+    (k : Z -> ctree E C X) (k' : Z -> ctree F D Y) L
+    {R : Chain (@sb E F C D X Y L)}
+    (HRask : Rask L e f)
+    (HRrcv : forall z, `R (k z) (k' z) /\ Rrcv L e f z z) :
+    sb L `R (Vis e k) (Vis f k').
+  Proof.
+    apply sb_vis; auto.
+    all: intros x; exists x; auto.
+  Qed.
+  
+  Lemma sbisim_vis_id {Z} (e : E Z) (f : F Z)
+    (k : Z -> ctree E C X) (k' : Z -> ctree F D Y) L
+    (HRask : Rask L e f)
+    (HRrcv : forall z, sbisim L (k z) (k' z) /\ Rrcv L e f z z) :
+    sbisim L (Vis e k) (Vis f k').
+  Proof.
+    now step; apply sb_vis_id.
+  Qed.
+  
+  (*|
+  Invisible branching — [Br]. Unlike [ss], the [_l]/[_r] variants require
+  an explicit witness so that the reverse challenge has a branch to take.
+  |*)
+  
+  Lemma sb_br_gen {A B} (c : C A) (d : D B)
+    (k : A -> ctree E C X) (k' : B -> ctree F D Y) R L :
+    (forall x, exists y, sb L R (k x) (k' y)) ->
+    (forall y, exists x, sb L R (k x) (k' y)) ->
+    sb L R (Br c k) (Br d k').
+  Proof.
+    intros EQs1 EQs2.
+    split; apply ss_br_gen; intros.
+    - destruct (EQs1 x) as [z [FW _]]. eauto.
+    - destruct (EQs2 x) as [z [_ BA]]. eauto.
+  Qed.
+  
+  Lemma sb_br_id_gen {A} (c : C A) (d : D A)
+    (k : A -> ctree E C X) (k' : A -> ctree F D Y) R L :
+    (forall x, sb L R (k x) (k' x)) ->
+    sb L R (Br c k) (Br d k').
+  Proof.
+    intros; apply sb_br_gen; intros x; exists x; auto.
+  Qed.
+
+  Lemma sb_br_l_gen {Z} (c : C Z) (x : Z)
+    (k : Z -> ctree E C X) (t : ctree F D Y) R L :
+    (forall z, sb L R (k z) t) ->
+    sb L R (Br c k) t.
+  Proof.
+    intros EQs.
+    split.
+    - apply ss_br_l_gen; intros; apply EQs.
+    - intros ?? TR.
+      eapply ss_br_r_gen with (x := x); eauto.
+      apply EQs.
+  Qed.
+
+  Lemma sb_br_r_gen {Z} (d : D Z) (y : Z)
+    (k : Z -> ctree F D Y) (t : ctree E C X) R L :
+    (forall z, sb L R t (k z)) ->
+    sb L R t (Br d k).
+  Proof.
+    intros EQs.
+    split.
+    - apply ss_br_r_gen with (x := y); intros; apply EQs.
+    - apply ss_br_l_gen; intros; apply EQs.
+  Qed.
+
+  Lemma sb_br {A B} (c : C A) (d : D B)
+    (k : A -> ctree E C X) (k' : B -> ctree F D Y) L
+    {R : Chain (@sb E F C D X Y L)} :
+    (forall x, exists y, sb L `R (k x) (k' y)) ->
+    (forall y, exists x, sb L `R (k x) (k' y)) ->
+    sb L `R (Br c k) (Br d k').
+  Proof.
+    now intros; apply sb_br_gen.
+  Qed.
+  
+  Lemma sb_br_id {A} (c : C A) (d : D A)
+    (k : A -> ctree E C X) (k' : A -> ctree F D Y) L
+    {R : Chain (@sb E F C D X Y L)} :
+    (forall x, sb L `R (k x) (k' x)) ->
+    sb L `R (Br c k) (Br d k').
+  Proof.
+    now intros; apply sb_br_id_gen.
+  Qed.
+
+  Lemma sb_br_l {Z} (c : C Z) (x : Z)
+    (k : Z -> ctree E C X) (t : ctree F D Y) L
+    {R : Chain (@sb E F C D X Y L)} :
+    (forall z, sb L `R (k z) t) ->
+    sb L `R (Br c k) t.
+  Proof.
+    now intros; apply sb_br_l_gen.
+  Qed.
+
+  Lemma sb_br_r {Z} (d : D Z) (y : Z)
+    (k : Z -> ctree F D Y) (t : ctree E C X) L
+    {R : Chain (@sb E F C D X Y L)} :
+    (forall z, sb L `R t (k z)) ->
+    sb L `R t (Br d k).
+  Proof.
+    now intros; apply sb_br_r_gen.
+  Qed.
+
+  Lemma sbisim_br {A B} (c : C A) (d : D B)
+    (k : A -> ctree E C X) (k' : B -> ctree F D Y) L :
+    (forall x, exists y, sbisim L (k x) (k' y)) ->
+    (forall y, exists x, sbisim L (k x) (k' y)) ->
+    sbisim L (Br c k) (Br d k').
+  Proof.
+    intros H1 H2; step; apply sb_br; eauto.
+    intros x; destruct (H1 x); eexists; step in H; eauto.
+    intros x; destruct (H2 x); eexists; step in H; eauto.
+  Qed.
+
+  Lemma sbisim_br_id {A} (c : C A) (d : D A)
+    (k : A -> ctree E C X) (k' : A -> ctree F D Y) L :
+    (forall x, sbisim L (k x) (k' x)) ->
+    sbisim L (Br c k) (Br d k').
+  Proof.
+    intros; step; apply sb_br_id; eauto.
+    intros x; specialize (H x); step in H; auto.
+  Qed.
+
+  Lemma sbisim_br_l {Z} (c : C Z) (x : Z)
+    (k : Z -> ctree E C X) (t : ctree F D Y) L :
+    (forall z, sbisim L (k z) t) ->
+    sbisim L (Br c k) t.
+  Proof.
+    intros; step; apply sb_br_l; eauto.
+    intros y; specialize (H y); step in H; auto.
+  Qed.
+
+  Lemma sbisim_br_r {Z} (d : D Z) (y : Z)
+    (k : Z -> ctree F D Y) (t : ctree E C X) L :
+    (forall z, sbisim L t (k z)) ->
+    sbisim L t (Br d k).
+  Proof.
+    intros; step; apply sb_br_r; eauto.
+    intros x; specialize (H x); step in H; auto.
+  Qed.
+
+  (* CHECKPOINT *)
+  (*|
+  Guard — a silent wrapper; absorbed by [≃].
+  |*)
+  Lemma sb_guard_l_gen (t : ctree E C X) (u : ctree F D Y) R L :
+    sb L R t u -> sb L R (Guard t) u.
+  Proof.
+    
+
+  Lemma sb_guard_l (t : ctree E C X) (u : ctree F D Y) L
+    {R : Chain (@sb E F C D X Y L)} :
+    sb L `R t u -> sb L `R (Guard t) u.
+  Admitted.
+
+  Lemma sbisim_guard_l (t : ctree E C X) (u : ctree F D Y) L :
+    sbisim L t u -> sbisim L (Guard t) u.
+  Admitted.
+
+  Lemma sb_guard_r_gen (t : ctree E C X) (u : ctree F D Y) R L :
+    sb L R t u -> sb L R t (Guard u).
+  Admitted.
+
+  Lemma sb_guard_r (t : ctree E C X) (u : ctree F D Y) L
+    {R : Chain (@sb E F C D X Y L)} :
+    sb L `R t u -> sb L `R t (Guard u).
+  Admitted.
+
+  Lemma sbisim_guard_r (t : ctree E C X) (u : ctree F D Y) L :
+    sbisim L t u -> sbisim L t (Guard u).
+  Admitted.
+
+  Lemma sbisim_guard (t : ctree E C X) (u : ctree F D Y) L :
+    sbisim L t u -> sbisim L (Guard t) (Guard u).
+  Admitted.
+
+  (*|
+  Internal transitions — [Step].
+  |*)
+  Lemma sb_step_gen (t : ctree E C X) (u : ctree F D Y) R L :
+    (Proper (Seq ==> Seq ==> impl) R) ->
+    L τ τ ->
+    R (α t) (α u) ->
+    sb L R (Step t) (Step u).
+  Admitted.
+
+  Lemma sb_step (t : ctree E C X) (u : ctree F D Y) L
+    {R : Chain (@sb E F C D X Y L)} :
+    L τ τ ->
+    `R t u ->
+    sb L `R (Step t) (Step u).
+  Admitted.
+
+  Lemma sbisim_step (t : ctree E C X) (u : ctree F D Y) L :
+    L τ τ ->
+    sbisim L t u ->
+    sbisim L (Step t) (Step u).
+  Admitted.
+
+  (*|
+  Visible branching — [BrS].
+  |*)
+  Lemma sb_brS {Z Z'} (c : C Z) (d : D Z')
+    (k : Z -> ctree E C X) (k' : Z' -> ctree F D Y) L
+    {R : Chain (@sb E F C D X Y L)} :
+    L τ τ ->
+    (forall x, exists y, `R (k x) (k' y)) ->
+    (forall y, exists x, `R (k x) (k' y)) ->
+    sb L `R (BrS c k) (BrS d k').
+  Admitted.
+
+  Lemma sbisim_brS {Z Z'} (c : C Z) (d : D Z')
+    (k : Z -> ctree E C X) (k' : Z' -> ctree F D Y) L :
+    L τ τ ->
+    (forall x, exists y, sbisim L (k x) (k' y)) ->
+    (forall y, exists x, sbisim L (k x) (k' y)) ->
+    sbisim L (BrS c k) (BrS d k').
+  Admitted.
+
+  Lemma sb_brS_id {Z} (c : C Z) (d : D Z)
+    (k : Z -> ctree E C X) (k' : Z -> ctree F D Y) L
+    {R : Chain (@sb E F C D X Y L)} :
+    L τ τ ->
+    (forall x, `R (k x) (k' x)) ->
+    sb L `R (BrS c k) (BrS d k').
+  Admitted.
+
+  Lemma sbisim_brS_id {Z} (c : C Z) (d : D Z)
+    (k : Z -> ctree E C X) (k' : Z -> ctree F D Y) L :
+    L τ τ ->
+    (forall x, sbisim L (k x) (k' x)) ->
+    sbisim L (BrS c k) (BrS d k').
+  Admitted.
+
+  (*|
+  [spinS] laws.
+  |*)
+  Lemma sbisim_spinS_nonempty :
+    forall {Z Z'} L (x : Z) (y : Z') (c : C Z) (c' : D Z'),
+      L τ τ ->
+      @sbisim E F C D X Y L (spinS_gen c) (spinS_gen c').
+  Admitted.
+
+  Lemma sbisim_spinS_empty :
+    forall L (c : C False) (c' : D False),
+      @sbisim E F C D X Y L (spinS_gen c) (spinS_gen c').
+  Admitted.
+
+(*|
+Inversion principles
+--------------------
+|*)
+
+  Lemma sbisim_stuck_inv L (t : ctree E C X) (u : ctree F D Y) :
+    sbisim L t u -> is_stuck t <-> is_stuck u.
+  Admitted.
+
+  Lemma sbisim_ret_l_inv L :
+    forall r (u : ctree F D Y),
+      sbisim L (Ret r : ctree E C X) u ->
+      exists r' u', trans (val r') u u' /\ RR L r r'.
+  Admitted.
+
+  Lemma sbisim_ret_r_inv L :
+    forall r' (t : ctree E C X),
+      sbisim L t (Ret r' : ctree F D Y) ->
+      exists r t', trans (val r) t t' /\ RR L r r'.
+  Admitted.
+
+  Lemma sbisim_ret_inv L (r : X) (r' : Y) :
+    sbisim L (Ret r : ctree E C X) (Ret r' : ctree F D Y) ->
+    RR L r r'.
+  Admitted.
+
+  Lemma sbisim_vis_l_inv {Z L} :
+    forall (e : E Z) (k : Z -> ctree E C X) u,
+      sbisim L (Vis e k) u ->
+      exists Z' (f : F Z') k',
+        trans (ask f) u (β f k') /\
+        Rask L e f /\
+        (forall x, exists y, sbisim L (k x) (k' y) /\ Rrcv L e f x y) /\
+        (forall y, exists x, sbisim L (k x) (k' y) /\ Rrcv L e f x y).
+  Admitted.
+
+  Lemma sbisim_vis_inv {Z Z'} L
+    (e : E Z) (f : F Z')
+    (k : Z -> ctree E C X) (k' : Z' -> ctree F D Y) :
+    sbisim L (Vis e k) (Vis f k') ->
+    Rask L e f /\
+    (forall x, exists y, Rrcv L e f x y /\ sbisim L (k x) (k' y)) /\
+    (forall y, exists x, Rrcv L e f x y /\ sbisim L (k x) (k' y)).
+  Admitted.
+
+  Lemma sbisim_vis_invT {Z Z'} L
+    (e : E Z) (f : F Z')
+    (k : Z -> ctree E C X) (k' : Z' -> ctree F D Y) (x : Z) :
+    sbisim L (Vis e k) (Vis f k') -> Rask L e f.
+  Admitted.
+
+  Lemma sbisim_guard_l_inv L (t : ctree E C X) (u : ctree F D Y) :
+    sbisim L (Guard t) u -> sbisim L t u.
+  Admitted.
+
+  Lemma sbisim_guard_r_inv L (t : ctree E C X) (u : ctree F D Y) :
+    sbisim L t (Guard u) -> sbisim L t u.
+  Admitted.
+
+  Lemma sbisim_guard_inv L (t : ctree E C X) (u : ctree F D Y) :
+    sbisim L (Guard t) (Guard u) -> sbisim L t u.
+  Admitted.
+
+  Lemma sbisim_br_l_inv L Z
+    (c : C Z) (t : ctree F D Y) (k : Z -> ctree E C X) :
+    sbisim L (Br c k) t ->
+    forall x, sbisim L (k x) t.
+  Admitted.
+
+  Lemma sbisim_br_r_inv L Z
+    (d : D Z) (t : ctree E C X) (k : Z -> ctree F D Y) :
+    sbisim L t (Br d k) ->
+    forall y, sbisim L t (k y).
+  Admitted.
+
+  Lemma sbisim_step_inv L (t : ctree E C X) (u : ctree F D Y) :
+    sbisim L (Step t) (Step u) -> sbisim L t u.
+  Admitted.
+
+  Lemma sbisim_step_l_inv L (t : ctree E C X) (u : ctree F D Y) :
+    sbisim L (Step t) u ->
+    exists u', trans τ u u' /\ sbisim L t u'.
+  Admitted.
+
+  Lemma sbisim_step_r_inv L (t : ctree E C X) (u : ctree F D Y) :
+    sbisim L t (Step u) ->
+    exists t', trans τ t t' /\ sbisim L t' u.
+  Admitted.
+
+  Lemma sbisim_brS_inv L
+    {A B} (c : C A) (d : D B)
+    (k1 : A -> ctree E C X) (k2 : B -> ctree F D Y) :
+    sbisim L (BrS c k1) (BrS d k2) ->
+    (forall a, exists b, sbisim L (k1 a) (k2 b)) /\
+    (forall b, exists a, sbisim L (k1 a) (k2 b)).
+  Admitted.
+
+  Lemma sbisim_brS_l_inv L
+    {A} (c : C A) (k1 : A -> ctree E C X) (u : ctree F D Y) :
+    sbisim L (BrS c k1) u ->
+    forall a, exists u', trans τ u u' /\ sbisim L (k1 a) u'.
+  Admitted.
+
+End Proof_Rules.
+
+(*|
+Sanity checks and structural laws (homogeneous).
+|*)
+Section WithParams.
+
+  Context {E C : Type -> Type}.
+  Context {HasC2 : B2 -< C}.
+  Context {HasC3 : B3 -< C}.
+
+  Lemma spin_bisim : forall {Z1 Z2} (c : C Z1) (c' : C Z2),
+      @spin_gen E C Z1 Z1 c ≃ @spin_gen E C Z2 Z2 c'.
+  Admitted.
+
+  Lemma br2_assoc {X} : forall (t u v : ctree E C X),
+      br2 (br2 t u) v ≃ br2 t (br2 u v).
+  Admitted.
+
+  Lemma br2_commut {X} : forall (t u : ctree E C X),
+      br2 t u ≃ br2 u t.
+  Admitted.
+
+  Lemma br2_idem {X} : forall (t : ctree E C X),
+      br2 t t ≃ t.
+  Admitted.
+
+  Lemma br2_merge {X} : forall (t u v : ctree E C X),
+      br2 (br2 t u) v ≃ br3 t u v.
+  Admitted.
+
+  Lemma br2_is_stuck {X} : forall (u v : ctree E C X),
+      is_stuck u -> br2 u v ≃ v.
+  Admitted.
+
+  Lemma br2_stuck_l {X} : forall (t : ctree E C X),
+      br2 Stuck t ≃ t.
+  Admitted.
+
+  Lemma br2_stuck_r {X} : forall (t : ctree E C X),
+      br2 t Stuck ≃ t.
+  Admitted.
+
+  Lemma br2_spin_l {X} : forall (t : ctree E C X),
+      br2 spin t ≃ t.
+  Admitted.
+
+  Lemma br2_spin_r {X} : forall (t : ctree E C X),
+      br2 t spin ≃ t.
+  Admitted.
+
+  Lemma brS2_commut {X} : forall (t u : ctree E C X),
+      brS2 t u ≃ brS2 u t.
+  Admitted.
+
+  Lemma brS2_idem {X} : forall (t : ctree E C X),
+      brS2 t t ≃ Step t.
+  Admitted.
+
+  Lemma sb_unfold_forever {X} : forall (k : X -> ctree E C X) (i : X),
+      forever k i ≃ r <- k i ;; forever k r.
+  Admitted.
+
+End WithParams.
+
+(*|
+Incompatibility lemmas — constructors of distinct kinds cannot be bisimilar
+(with minor inhabitation side-conditions for stuck [Vis] cases).
+|*)
+Section Incompat.
+
+  Context {E C : Type -> Type}.
+
+  Definition are_bisim_incompat {X} (t u : ctree E C X) : Type :=
+    match observe t, observe u with
+    | RetF _, RetF _
+    | VisF _ _, VisF _ _
+    | BrF _ _, _
+    | _, BrF _ _
+    | GuardF _, _
+    | _, GuardF _
+    | StepF _, StepF _
+    | StuckF, StuckF => False
+    | @VisF _ _ _ _ Z _ _, StuckF
+    | StuckF, @VisF _ _ _ _ Z _ _ => inhabited Z
+    | _, _ => True
+    end.
+
+  Lemma sbisim_absurd {X} (t u : ctree E C X) :
+    are_bisim_incompat t u -> t ≃ u -> False.
+  Admitted.
+
+  Lemma sbisim_ret_vis_inv {X Y} (r : Y) (e : E X) (k : X -> ctree E C Y) :
+    (Ret r : ctree E C _) ≃ Vis e k -> False.
+  Admitted.
+
+  Lemma sbisim_ret_BrS_inv {X Y} (r : Y) (c : C X) (k : X -> ctree E C Y) :
+    (Ret r : ctree E C _) ≃ BrS c k -> False.
+  Admitted.
+
+  Lemma sbisim_vis_BrS_inv {X Y Z}
+    (e : E X) (k1 : X -> ctree E C Z) (c : C Y) (k2 : Y -> ctree E C Z) (y : Y) :
+    Vis e k1 ≃ BrS c k2 -> False.
+  Admitted.
+
+  Lemma sbisim_vis_BrS_inv' {X Y Z}
+    (e : E X) (k1 : X -> ctree E C Z) (c : C Y) (k2 : Y -> ctree E C Z) (x : X) :
+    Vis e k1 ≃ BrS c k2 -> False.
+  Admitted.
+
+End Incompat.
+
+(*|
+Interaction with (complete) strong simulation
+=============================================
+|*)
+Section SBisim_vs_SSim.
+
+  Context {E F C D : Type -> Type} {X Y : Type}
+          {L : lrel E F X Y}.
+
+  Notation ss    := (@ss    E F C D X Y).
+  Notation ssim  := (@ssim  E F C D X Y).
+
+  (*|
+  A two-sided [ss] gives an [sb]; the converse fails in general (see
+  [ssim_sbisim_nequiv] below).
+  |*)
+  Lemma ss_sb (R : rel _ _) (t : ctree E C X) (u : ctree F D Y) :
+    ss L R t u ->
+    ss (flipL L) (flip R) u t ->
+    sb L R t u.
+  Admitted.
+
+  Lemma sbisim_clos_ss {c : Chain (ss L)} :
+    forall x y, @sbisim_clos E F C D X Y Leq Leq `c x y -> `c x y.
+  Admitted.
+
+  #[global] Instance sbisim_eq_clos_ss_goal {R : Chain (ss L)} :
+    Proper (sbisim Leq ==> sbisim Leq ==> flip impl) `R.
+  Admitted.
+
+  #[global] Instance sbisim_eq_clos_ss_ctx {R : Chain (ss L)} :
+    Proper (sbisim Leq ==> sbisim Leq ==> impl) `R.
+  Admitted.
+
+  #[global] Instance sbisim_eq_clos_ssim_goal :
+    Proper (sbisim Leq ==> sbisim Leq ==> flip impl) (ssim L).
+  Admitted.
+
+  #[global] Instance sbisim_eq_clos_ssim_ctx :
+    Proper (sbisim Leq ==> sbisim Leq ==> impl) (ssim L).
+  Admitted.
+
+End SBisim_vs_SSim.
+
+Section Two_ss_is_not_sb.
+
+  (*|
+  Two [ssim]s do not always give an [sbisim] (witness below).
+  |*)
+  Lemma split_sb_eq {E C X} (RR : rel _ _) (t t' : ctree E C X) :
+    ss Leq RR t t' ->
+    ss Leq (flip RR) t' t ->
+    sb Leq RR t t'.
+  Admitted.
+
+  Lemma split_sbisim_eq {E B X} (t u : ctree E B X) :
+    t ≃ u <-> ss Leq (sbisim Leq) t u /\ ss Leq (sbisim Leq) u t.
+  Admitted.
+
+  (*|
+  A concrete counter-example: [Step (Ret tt)] and [brS2 (Ret tt) Stuck]
+  are mutually [ssim]-related but not [sbisim]-related.
+  |*)
+  Lemma ssim_sbisim_nequiv :
+    exists (t1 t2 : ctree void1 B2 unit),
+      ssim Leq t1 t2 /\ ssim Leq t2 t1 /\ ≃ sbisim Leq t1 t2.
+  Admitted.
+
+End Two_ss_is_not_sb.
+
+Section SBisim_vs_CSSim.
+
+  Context {E F C D : Type -> Type} {X Y : Type}
+          {L : lrel E F X Y}.
+
+  Notation css   := (@css   E F C D X Y).
+  Notation cssim := (@cssim E F C D X Y).
+
+  Lemma sb_css (R : rel _ _) (t : ctree E C X) (u : ctree F D Y) :
+    sb L R t u -> css L R t u.
+  Admitted.
+
+  Lemma css_sb (R : rel _ _) (t : ctree E C X) (u : ctree F D Y) :
+    css L R t u ->
+    css (flipL L) (flip R) u t ->
+    sb L R t u.
+  Admitted.
+
+  Lemma sbisim_clos_css {c : Chain (css L)} :
+    forall x y, @sbisim_clos E F C D X Y Leq Leq `c x y -> `c x y.
+  Admitted.
+
+  #[global] Instance sbisim_eq_clos_css_goal {R : Chain (css L)} :
+    Proper (sbisim Leq ==> sbisim Leq ==> flip impl) `R.
+  Admitted.
+
+  #[global] Instance sbisim_eq_clos_css_ctx {R : Chain (css L)} :
+    Proper (sbisim Leq ==> sbisim Leq ==> impl) `R.
+  Admitted.
+
+  #[global] Instance sbisim_eq_clos_cssim_goal :
+    Proper (sbisim Leq ==> sbisim Leq ==> flip impl) (cssim L).
+  Admitted.
+
+  #[global] Instance sbisim_eq_clos_cssim_ctx :
+    Proper (sbisim Leq ==> sbisim Leq ==> impl) (cssim L).
+  Admitted.
+
+End SBisim_vs_CSSim.
