theories/Utils/coinduction_addon.v
@@ -1,0 +1,34 @@
+(*
+Convenience to step/unstep in relations built using the coinduction library.
+Hopefully upstreamed eventually: https://github.com/damien-pous/coinduction/pull/22
+ *)
+
+From Coinduction Require Import all.
+
+Lemma pfp_gfp {X : Type} {L : CompleteLattice X} (b : mon X) : b (gfp b) <= gfp b.
+Proof. apply b_chain. Qed.
+
+Ltac step :=
+match goal with
+| |- context [gfp ?b] => apply (pfp_gfp b)
+| |- context [elem ?R] => apply (b_chain R)
+end.
+
+Ltac step_in h :=
+match type of h with
+| context [gfp ?b] => apply (gfp_pfp b) in h
+end.
+
+Tactic Notation "step" "in" ident(h) := step_in h.
+
+Ltac unstep :=
+match goal with
+| |- context [gfp ?b] => apply (gfp_pfp b)
+end.
+
+Ltac unstep_in h :=
+match type of h with
+| context [gfp ?b] => apply (pfp_gfp b) in h
+end.
+
+Tactic Notation "unstep" "in" ident(h) := unstep_in h.
